Add test for mint and transfer method

test/test_transfer.dfy
@@ -1,32 +1,202 @@
-include "../token/token.dfy"
+include "../utils/NonNativeTypes.dfy"
 
-predicate GInv(totalAmount:nat, balances:map<Address, uint256>) 
-{
-    totalAmount == sum(balances)
+module test_GInv_Provability {
+    import opened NonNativeTypes
+
+    datatype Account = Account(balance:uint256, isContract:bool)
+    datatype Msg = Msg(sender: Account, value: uint256) 
+
+
+    type Address = Account
+
+    function mapSum(m:map<Address, uint256>):nat
+    {
+        if |m| == 0 then 0 else
+        var a :| a in m.Keys;
+        var mapLess:map<Address, uint256> := map key | key in m.Keys && key != a :: m[key];
+        m[a] as nat + mapSum(mapLess)
+    }
+
+    function sum(m: map<Address, uint256>): nat
+        ensures m == map[] ==> sum(m) == 0
+    {
+        mapSum(m)
+    }
+
+    predicate GInv(totalAmount:nat, balances:map<Address, uint256>) {
+        totalAmount == sum(balances)
+    }
+
+    predicate pre_transfer(from:Address, to:Address, amount:uint256, msg:Msg, gas:nat, balances:map<Address, uint256>, totalAmount:nat)
+    {
+        && from in balances
+        && gas >= 1
+        && msg.value == 0
+        && balances[from] >= amount && msg.sender == from 
+        && (to !in balances ||  balances[to] as nat + amount as nat <= MAX_UINT256)
+        && msg.sender == from  
+        && GInv(totalAmount, balances)
+    }
+
+    predicate post_transfer(from:Address, to:Address, amount:uint256, msg:Msg, gas:nat, gas':nat, balances:map<Address, uint256>, balances':map<Address, uint256>, totalAmount:nat, totalAmount':nat)
+        requires pre_transfer(from, to, amount, msg, gas, balances, totalAmount)
+    {
+        && GInv(totalAmount', balances')
+        && from in balances' && balances'[from] == (balances[from]) - amount
+        && to in balances'
+        && (to != from ==> balances'[to] >= amount)
+        && (to == from ==> balances' == (balances))
+        && gas' < gas
+    }
+
+    lemma test_pre_transfer_usefulness(from:Address, to:Address, amount:uint256, msg:Msg, gas:nat, balances:map<Address, uint256>, totalAmount:nat)
+        requires from == Account(100, false)
+        requires amount == 10
+        requires balances == map[Account(100, false) := 10]
+        requires gas > 0
+        requires msg.sender == from
+        requires msg.value == 0
+        requires totalAmount == 10
+        ensures pre_transfer(from, to, amount, msg, gas, balances,totalAmount)
+    {
+        assert sum(map[Account(100, false) := 10]) == 10;
+        assert balances[from] >= amount;
+    }
+
+    lemma test_pre_transfer_provability(from:Address, to:Address, amount:uint256, msg:Msg, gas:nat, balances:map<Address, uint256>, totalAmount:nat)
+        requires from == Account(100, false)
+        requires amount > 10
+        requires balances == map[Account(100, false) := 10]
+        requires gas > 0
+        requires msg.sender == from
+        requires msg.value == 0
+        requires totalAmount == 10
+        ensures !pre_transfer(from, to, amount, msg, gas, balances,totalAmount)
+    {}
+
+    lemma test_post_transfer_correctness_1(from:Address, to:Address, amount:uint256, msg:Msg, gas:nat, gas':nat, balances:map<Address, uint256>, balances':map<Address, uint256>, totalAmount:nat, totalAmount':nat)
+        requires from == Account(100, false)
+        requires amount == 10
+        requires balances == map[Account(100, false) := 10]
+        requires gas > 0
+        requires msg.sender == from
+        requires msg.value == 0
+        requires totalAmount == 10
+        requires pre_transfer(from, to, amount, msg, gas, balances,totalAmount)
+        requires post_transfer(from, to, amount, msg, gas, gas', balances, balances', totalAmount, totalAmount')
+        ensures totalAmount' == 10
+    {
+        assert sum(map[Account(100, false) := 10]) == 10;
+
+        assert balances' == map[Account(100, false) := 0, to := 10];
+        // not able to prove ==> look at the specification ==> find a counter example below
+        
+        assert mapSum(balances') == mapSum(map[to:=10]) + 0;
+        assert sum(balances') == 10; 
+    }
+
+    lemma test_post_transfer_correctness_1_counterexample(from:Address, to:Address, amount:uint256, msg:Msg, gas:nat, gas':nat, balances:map<Address, uint256>, balances':map<Address, uint256>, totalAmount:nat, totalAmount':nat)
+        requires from == Account(100, false)
+        requires amount == 10
+        requires balances == map[Account(100, false) := 10]
+        requires gas > 0
+        requires msg.sender == from
+        requires msg.value == 0
+        requires totalAmount == 10
+        requires totalAmount' == 11
+        requires to == Account(50, false)
+        requires gas' == gas - 1
+        requires balances' == map[Account(100, false) := 0, to := 10, Account(25, false):= 1]
+        ensures pre_transfer(from, to, amount, msg, gas, balances,totalAmount)
+        ensures post_transfer(from, to, amount, msg, gas, gas', balances, balances', totalAmount, totalAmount')
+    {
+        assert sum(map[Account(100, false) := 10]) == 10;
+
+        assert map[Account(100, false) := 0, to := 10, Account(25, false):= 1][Account(100, false)] == 0;
+        assert Account(100, false) in balances';
+        var mapLess:map<Address, uint256> := map key | key in balances'.Keys && key != Account(100, false) :: balances'[key];
+        assert mapLess == map[to := 10, Account(25, false):= 1];
+        assert mapSum(balances') == 0 + mapSum(map[to := 10, Account(25, false):= 1]);
+        assert mapSum(map[to := 10, Account(25, false):= 1]) == 10 + mapSum(map[Account(25, false):= 1]);
+        assert sum(balances') == 11; 
+    }
+
+    lemma test_post_transfer_correctness_2(from:Address, to:Address, amount:uint256, msg:Msg, gas:nat, gas':nat, balances:map<Address, uint256>, balances':map<Address, uint256>, totalAmount:nat, totalAmount':nat)
+        requires from == Account(100, false)
+        requires amount == 5
+        requires balances == map[Account(100, false) := 10]
+        requires gas > 0
+        requires msg.sender == from
+        requires msg.value == 0
+        requires totalAmount == 10
+        requires gas' != gas - 1
+        ensures pre_transfer(from, to, amount, msg, gas, balances,totalAmount)
+        ensures !post_transfer(from, to, amount, msg, gas, gas', balances, balances', totalAmount, totalAmount')
+    {
+        assert sum(map[Account(100, false) := 10]) == 10;
+        
+        // not able to prove ==> see specification ==> directly find that it does not explicitly say that gas must -1
+    }
+
+    lemma test_post_transfer_correctness_3(from:Address, to:Address, amount:uint256, msg:Msg, gas:nat, gas':nat, balances:map<Address, uint256>, balances':map<Address, uint256>, totalAmount:nat, totalAmount':nat)
+        requires from == Account(100, false)
+        requires amount == 5
+        requires balances == map[Account(100, false) := 10]
+        requires gas > 0
+        requires msg.sender == from
+        requires msg.value == 0
+        requires totalAmount == 10
+        requires balances' != map[Account(100, false) := 5, to := 5]
+        ensures pre_transfer(from, to, amount, msg, gas, balances,totalAmount)
+        ensures !post_transfer(from, to, amount, msg, gas, gas', balances, balances', totalAmount, totalAmount')
+    {
+        assert sum(map[Account(100, false) := 10]) == 10;
+        // not able to prove ==> look at the specification ==> find a counter example below
+
+    }
+
+    lemma test_post_transfer_correctness_3_counterexample(from:Address, to:Address, amount:uint256, msg:Msg, gas:nat, gas':nat, balances:map<Address, uint256>, balances':map<Address, uint256>, totalAmount:nat, totalAmount':nat)
+        requires from == Account(100, false)
+        requires amount == 5
+        requires balances == map[Account(100, false) := 10]
+        requires gas > 0
+        requires msg.sender == from
+        requires msg.value == 0
+        requires totalAmount == 10
+        requires totalAmount' == 15
+        requires to == Account(50, false)
+        requires gas' == gas - 1
+        requires balances' == map[Account(100, false) := 5, to := 5, Account(25, false):= 5]
+
+        ensures pre_transfer(from, to, amount, msg, gas, balances,totalAmount)
+        ensures post_transfer(from, to, amount, msg, gas, gas', balances, balances', totalAmount, totalAmount')
+    {
+        assert sum(map[Account(100, false) := 10]) == 10;
+
+        assert Account(100, false) in balances';
+        var mapLess:map<Address, uint256> := map key | key in balances'.Keys && key != Account(100, false) :: balances'[key];
+        assert mapLess == map[to := 5, Account(25, false):= 5];
+        assert mapSum(balances') == 5 + mapSum(map[to := 5, Account(25, false):= 5]);
+        assert mapSum(map[to := 5, Account(25, false):= 5]) == 5 + mapSum(map[Account(25, false):= 5]);
+        assert sum(balances') == 15; 
+    }
+
+    lemma test_post_transfer_provability_1(from:Address, to:Address, amount:uint256, msg:Msg, gas:nat, gas':nat, balances:map<Address, uint256>, balances':map<Address, uint256>, totalAmount:nat, totalAmount':nat)
+        requires from == Account(100, false)
+        requires amount == 5
+        requires balances == map[Account(100, false) := 10]
+        requires gas > 0
+        requires msg.sender == from
+        requires msg.value == 0
+        requires totalAmount == 10
+        requires totalAmount' == 10
+        requires to == Account(50, false)
+        requires gas' == gas - 1
+        requires balances' == map[Account(100, false) := 5, to := 5]
+        ensures pre_transfer(from, to, amount, msg, gas, balances,totalAmount)
+        ensures post_transfer(from, to, amount, msg, gas, gas', balances, balances', totalAmount, totalAmount')
+    {
+        assert sum(map[Account(100, false) := 10]) == 10;
+        assert mapSum(map[Account(100, false) := 5, to := 5]) == 5 + mapSum(map[to:=5]);
+    }
 }
-
-predicate pre_transfer(totalAmount:nat, balances: map<Address, uint256>, from: Address, to: Address, amount: uint256, msg: Msg, gas: nat)
-{
-    && (from in balances)
-    && gas >= 1
-    && msg.value == 0
-    && balances[from] >= amount && msg.sender == from 
-    && (to !in balances ||  balances[to] as nat + amount as nat <= MAX_UINT256)
-    && msg.sender == from  
-    && GInv(totalAmount, balances)
-}
-
-predicate post_transfer(totalAmount:nat, balances: map<Address, uint256>, from: Address, to: Address, amount: uint256, msg: Msg, gas: nat, g:nat, balances':map<Address, uint256>, totalAmount':nat)
-    requires pre_transfer(totalAmount, balances, from, to, amount, msg, gas)
-{
-    && GInv(totalAmount, balances')
-    && from in balances' && balances'[from] == balances[from] - amount
-    && to in balances' 
-    && (to != from ==> balances'[to] >= amount)
-    && (to == from ==> balances' == balances)
-}
-
-// // usefulness: precondition
-// lemma test_pre_usefulness_1(totalAmount:nat, balances: map<Address, uint256>, from: Address, to: Address, amount: uint256, msg: Msg, gas: nat)
-//     requires totalAmount == 100
-//     requires balances == map[Account:= 100]
