test/test_mint.dfy
@@ -1,0 +1,83 @@
+include "../utils/NonNativeTypes.dfy"
+
+module test_GInv_Provability {
+    import opened NonNativeTypes
+
+    datatype Account = Account(balance:uint256, isContract:bool)
+    datatype Msg = Msg(sender: Account, value: uint256) 
+
+    type Address = Account
+
+    function mapSum(m:map<Address, uint256>):nat
+    {
+        if |m| == 0 then 0 else
+        var a :| a in m.Keys;
+        var mapLess:map<Address, uint256> := map key | key in m.Keys && key != a :: m[key];
+        m[a] as nat + mapSum(mapLess)
+    }
+
+    function sum(m: map<Address, uint256>): nat
+        ensures m == map[] ==> sum(m) == 0
+    {
+        mapSum(m)
+    }
+
+    predicate GInv(totalAmount:nat, balances:map<Address, uint256>) {
+        totalAmount == sum(balances)
+    }
+
+    predicate pre_mint(to:Address, amount:uint256, minter:Address, msg:Msg, gas:nat, balances:map<Address, uint256>, totalAmount:nat) {
+        && msg.sender == minter
+        && gas >= 1
+        && (to !in balances ||  balances[to] as nat + amount as nat <= MAX_UINT256)
+        && GInv(totalAmount, balances)
+    }
+
+    predicate post_mint(to:Address, amount:uint256, minter:Address, msg:Msg, gas:nat, gas':nat, balances:map<Address, uint256>, balances':map<Address, uint256>, totalAmount:nat, totalAmount':nat) {
+        && totalAmount' == (totalAmount) + amount as nat
+        && GInv(totalAmount', balances')
+    }
+
+    lemma test_pre_mint_usefulness(to:Address, amount:uint256, minter:Address, msg:Msg, gas:nat, balances:map<Address, uint256>, totalAmount:nat)
+        requires minter == Account(100, false)
+        requires msg.sender == minter
+        requires gas == 1
+        requires amount as nat == MAX_UINT256
+        requires to !in balances
+        requires GInv(totalAmount, balances)
+        ensures pre_mint(to, amount, minter, msg, gas, balances, totalAmount)
+    {}
+
+    lemma test_pre_mint_provability(to:Address, amount:uint256, minter:Address, msg:Msg, gas:nat, balances:map<Address, uint256>, totalAmount:nat)
+        requires gas == 0 || msg.sender != minter
+        ensures !pre_mint(to, amount, minter, msg, gas, balances, totalAmount)
+    {}
+
+    lemma test_post_mint_correctness(to:Address, amount:uint256, minter:Address, msg:Msg, gas:nat, gas':nat, balances:map<Address, uint256>, balances':map<Address, uint256>, totalAmount:nat, totalAmount':nat)
+        requires to == Account(100, false)
+        requires balances == map[]
+        requires amount == 100
+        requires balances' == map[Account(50, false) := 100]
+        requires pre_mint(to, amount, minter, msg, gas, balances, totalAmount)
+        ensures !post_mint(to, amount, minter, msg, gas, gas', balances, balances', totalAmount, totalAmount')
+    {
+        assert to !in balances';
+        // not able to prove ==> look at the specification ==> confident that this is a bug
+    }
+
+    lemma test_post_mint_provability(to:Address, amount:uint256, minter:Address, msg:Msg, gas:nat, gas':nat, balances:map<Address, uint256>, balances':map<Address, uint256>, totalAmount:nat, totalAmount':nat)
+        requires to == Account(100, false)
+        requires balances == map[]
+        requires totalAmount == 0
+        requires amount == 100
+        requires balances' == map[Account(100, false) := 100]
+        requires totalAmount' == 100;
+        requires minter == msg.sender
+        requires gas == 1
+        ensures pre_mint(to, amount, minter, msg, gas, balances, totalAmount)
+        ensures post_mint(to, amount, minter, msg, gas, gas', balances, balances', totalAmount, totalAmount')
+    {}
+
+
+
+}
